
R(u, v) - (1/2)g(u,v) x R(t) + I x g(u,v) = G(u,v)xT(u, v)

I = cosmical constant
G = einstein gravity constant in gravity mechanics of mc^2 >= mgh and g <= 8pi * G / c^4
g = newton gravity constant in classical mechanics of mgh >= (1/2)mv^2 >= (1/2)t^2 >= 0 for mass of atoms
c = bohr gravity constant in quantum mechanics of electron and photon energy in an atom
S = bubble of spacetime
dS/dt = curve of spacetime
N = bubble of light
dN/dt = particles of 2 lights in m(t)

N(t) = dS/dt
S(t) = N(t) / t

proving time as 1 second
1 second of 1 electron velocity and 1 photon velocity as light mass
1 second of thermal light mass in electron relationships with atoms and particles
1 second of all light mass in relationship to all gravity in spacetime

Idea: What if light mass is the result of curved spacetime as time bubble of photons and electrons at speeds of light
Then you suggest time bubbles as light bubbles to space bubbles over time in nexus bubble?